
\section{Methods}\label{sec:methods}



\Nanna{choose one of these:}
\begin{equation}\label{eq:p4_initial_condition}
\begin{split}
    u(t\!=\!0, \vec{x}) = & \exp{-(\vec{x}-\vec{x}_\mathrm{c})^\mathrm{T}\Sigma^{-1}(\vec{x}-\vec{x}_\mathrm{c}) + \im \vec{p}^\mathrm{T}(\vec{x}-\vec{x}_\mathrm{c})} \,;  \\ 
    &\quad\Sigma = \mathrm{diag}(\svec{\sigma}^2) 
\end{split}
\end{equation}

\begin{equation}\label{eq:p4_initial_condition_scalarform}
    u(t\!=\!0, \vec{x}) = \exp{-\frac{(x-x_\mathrm{c})^2}{2\sigma_x^2} -\frac{(y-y_\mathrm{c})^2}{2\sigma_y^2} + \im \vec{p}\cdot (\vec{x}-\vec{x}_\mathrm{c})}
\end{equation}

% ===========================================
